\documentclass{article}
\usepackage{amsmath}
\usepackage{amssymb}
\usepackage{graphicx}
\usepackage{float}
\usepackage{hyperref}
\usepackage{fancyvrb}
\usepackage{matlab-prettifier}
\setlength{\parindent}{0pt}
\graphicspath{{../images/}}

\title{CS663: Digital Image Processing - Homework 3}
\author{Harsh $\vert$ Pranav $\vert$ Swayam} 
\date{October 1, 2024}

\begin{document}

\maketitle
\section{Homework 3 - Question 5}
We have,
$$
F(u,v) = \sum_{x,y} f(x,y) \exp\left(-j 2 \pi \frac{(ux + vy)}{N}\right)
$$
$$
F(-u,-v) = \sum_{x,y} f(x,y) \exp\left(j 2 \pi \frac{(ux + vy)}{N}\right).
$$
\begin{equation}
\begin{split}
\therefore F^*(u,v) &= \left( \sum_{x,y} f(x,y) \exp\left(-j 2 \pi \frac{(ux + vy)}{N}\right) \right)^* \\
&= F(-u,-v)
\end{split}
\end{equation}
\texttt{The conjugation step is valid because $f(x,y)$ is real-valued}.
\vspace{10pt}

If $f$ is both real and even, i.e. $f(x,y) = f(-x,-y)$. Then we have:
\begin{equation}
\begin{split}
F^*(u,v) &= \left( \sum_{x=0}^{N} \sum_{y=0}^{N} f(x,y) \exp\left(-j 2 \pi \frac{(ux + vy)}{N}\right) \right)^*\\
&= \sum_{x=0}^{N} \sum_{y=0}^{N} f(x,y) \exp\left(j 2 \pi \frac{(ux + vy)}{N}\right) \\
&= \sum_{x=0}^{N} \sum_{y=0}^{N} f(-x,-y) \exp\left(j 2 \pi \frac{(-ux - vy)}{N}\right)
\end{split}
\end{equation}
By substituting $x' = -x$ and $y' = -y$, we get -
$$
= \sum_{x'=0}^{N} \sum_{y'=0}^{N} f(x',y') \exp\left(-j 2 \pi \frac{(ux' + vy')}{N}\right)
$$
\begin{equation}
= F(u,v)
\end{equation}
Hence, $F(u,v)$ is proven to be real-valued. 

\vspace{10pt}
We already proved $F^*(u,v) = F(-u,-v)$ which in this case shows that $F(u,v) = F(-u,-v)$ and hence $F(u,v)$ is even.

Therefore, if $f$ is real and even, then $F(u,v)$ is also real and even.

\end{document}